# Odd Integers

## Definition

n is odd ⇒ (∃m ∈ ℤ)(n = 2m + 1)

## Practices

1. Prove that the sum of any two odd integers is an even.

## Answers

1. Suppose x and y be odd numbers.

<table>
  <tr>
    <td>∃m : x = 2m + 1 and ∃n : y = 2n + 1</td>
    <td><i>Definition of odd integer</i></td>
  </tr>
  <tr>
    <td>⇒ x + y = 2m + 1 + 2n + 1</td>
    <td><i>?</i></td>
  </tr>
  <tr>
    <td>= 2(m + n + 1)</td>
    <td><i>Definition of even integer</i></td>
  </tr>
</table>

Therefore, according to the definition of even integer, x + y, the sum of any two odd integers, is even. 