# Induction Proving Method

## Definition

## Examples

## Practices

1. Prove that if ğ‘› â‰¥ ğŸ¶, ğ‘†ğ‘¢ğ‘š(ğ¶(ğ‘›, ğ‘˜), (ğ‘˜, ğŸ¶, ğ‘›)) = ğŸ¸<sup>ğ‘›</sup>

## Answers

1. ğ‘› = ğŸ¶, (ğŸ¶ ğŸ¶) = ğŸ· = ğŸ¸<sup>ğŸ¶</sup><br>
ğ‘› = ğŸ·, (ğŸ· ğŸ¶) + (ğŸ· ğŸ·) = ğŸ¸ = ğŸ¸<sup>ğŸ·</sup><br>
ğ‘› = ğŸ¸, (ğŸ¸ ğŸ¶) + (ğŸ¸ ğŸ·) + (ğŸ¸ ğŸ¸) = ğŸº = ğŸ¸<sup>ğŸ¸</sup>

Assume ğ‘†ğ‘¢ğ‘š(ğ¶(ğ‘›, ğ‘˜), (ğ‘˜, ğŸ¶, ğ‘›)) = ğŸ¸<sup>ğ‘›</sup> is true,<br>
- ğ‘†ğ‘¢ğ‘š(ğ¶(ğ‘›, ğ‘˜), (ğ‘˜, ğŸ¶, ğ‘›)) + ğ‘†ğ‘¢ğ‘š(ğ¶(ğ‘›, ğ‘˜), (ğ‘˜, ğŸ¶, ğ‘›)) = ğŸ¸<sup>ğ‘›</sup> + ğŸ¸<sup>ğ‘›</sup> = ğŸ¸<sup>ğ‘›+ğŸ·</sup> (1)
- Shifting one place to right and applying Binomial Coefficient Formula for each pair, ğ‘†ğ‘¢ğ‘š(ğ¶(ğ‘›, ğ‘˜), (ğ‘˜, ğŸ¶, ğ‘›)) + ğ‘†ğ‘¢ğ‘š(ğ¶(ğ‘›, ğ‘˜), (ğ‘˜, ğŸ¶, ğ‘›)) = ğ‘†ğ‘¢ğ‘š(ğ¶(ğ‘›+1, ğ‘˜), (ğ‘˜, ğŸ¶, ğ‘›+1)) since (ğ‘› ğŸ¶) = (ğ‘›+ğŸ· ğŸ¶) and (ğ‘›, ğ‘›) = (ğ‘›+ğŸ·, ğ‘›+ğŸ·)

Thus, ğ‘†ğ‘¢ğ‘š(ğ¶(ğ‘›+1, ğ‘˜), (ğ‘˜, ğŸ¶, ğ‘›+1)) = ğŸ¸<sup>ğ‘›+ğŸ·</sup>.

In conclusion, ğ‘†ğ‘¢ğ‘š(ğ¶(ğ‘›, ğ‘˜), (ğ‘˜, ğŸ¶, ğ‘›)) = ğŸ¸<sup>ğ‘›</sup>