# Solving Recurrence Relations

## Examples

### 洧녩<sub>洧녵</sub> = 洧맂洧녩<sub>洧녵-洧링</sub>

Since it's a description of a geometric sequence, 洧녩<sub>洧녵</sub> = 洧녩<sub>洧맀</sub>洧맂<sup>洧녵</sup>.

### 洧녩<sub>洧녵</sub> = 洧맂洧녩<sub>洧녵-洧링</sub> + 洧맅
洧녩<sub>洧링</sub> = 洧맂洧녩<sub>洧맀</sub> + 洧맅<br>
洧녩<sub>洧맂</sub> = 洧맂(洧맂洧녩<sub>洧맀</sub> + 洧맅) + 洧맅 = 洧맄洧녩<sub>洧맀</sub> + (洧맃)洧맅<br>
洧녩<sub>洧맃</sub> = 洧맂(洧맄洧녩<sub>洧맀</sub> + (洧맃)洧맅) + 洧맅 = 洧쮫롐<sub>洧맀</sub> + (洧맇)洧맅<br>
洧녩<sub>洧맄</sub> = 洧맂(洧쮫롐<sub>洧맀</sub> + (洧맇)洧맅) + 洧맅 = 洧링洧맆洧녩<sub>洧맀</sub> + (洧링洧맅)洧맅<br>

We can guess 洧녩<sub>洧녵</sub> = 洧맂<sup>洧녵</sup>洧녩<sub>洧맀</sub> + (洧맂<sup>洧녵</sup>-洧링)洧맅 (1)

Assuming (1) is right, substituting it as 洧녩<sub>洧녵-洧링</sub><br>
洧녩<sub>洧녵</sub> = 洧맂洧녩<sub>洧녵-洧링</sub> + 洧맅<br>
= 洧맂(洧맂<sup>洧녵-洧링</sup>洧녩<sub>洧맀</sub> + (洧맂<sup>洧녵-洧링</sup>-洧링)洧맅) + 洧맅<br>
= 洧맂<sup>洧녵</sup>洧녩<sub>洧맀</sub> + (洧맂<sup>洧녵</sup>-洧링)洧맅<br>
= 洧녩<sub>洧녵</sub>

Therefore, 洧녩<sub>洧녵</sub> = 洧맂<sup>洧녵</sup>洧녩<sub>洧맀</sub> + (洧맂<sup>洧녵</sup>-洧링)洧맅

### 洧녩<sub>洧녵</sub> = 洧맂洧녩<sub>洧녵-洧링</sub> - 洧녩<sub>洧녵-洧맂</sub>

洧녩<sub>洧녵</sub> - 洧맂洧녩<sub>洧녵-洧링</sub> + 洧녩<sub>洧녵-洧맂</sub> = 洧맀

洧녹洧논<sub>洧링</sub><sup>洧녵</sup> + 洧녺洧논<sub>洧맂</sub><sup>洧녵</sup><br>
(洧녹 + 洧녺洧녵)洧논<sup>洧녵</sup>