# Binomial Coefficients

## Definitions

### Recursion version

Assume 𝑛 ≥ 𝑘 ≥ 𝟶. We define (𝑛 𝑘) by
- (𝑛 𝟶) = 𝟷
- (𝑛 𝑛) = 𝟷 and
- (𝑛 𝑘) = (𝑛-𝟷 𝑘) + (𝑛-𝟷 𝑘-𝟷) if 𝑛 > 𝑘 > 𝟶

## Practices

1. Expanding (𝟽 𝟸)

## Answers

1. (𝟽 𝟸) = (𝟼 𝟸) + (𝟼 𝟷)<br>
= (𝟻 𝟸) + (𝟻 𝟷) + (𝟻 𝟷) + (𝟻 𝟶) = (𝟻 𝟸) + 𝟸(𝟻 𝟷) + 𝟷<br>
= (𝟺, 𝟸) + (𝟺 𝟷) + 𝟸(𝟺 𝟷) + 𝟸(𝟺 𝟶) + 1 = (𝟺 𝟸) + 𝟹(𝟺 𝟷) + 𝟹<br>
= (𝟹 𝟸) + (𝟹 𝟷) + 𝟹(𝟹 𝟷) + 𝟹(𝟹 𝟶) + 𝟹 = (𝟹 𝟸) + 𝟺(𝟹 𝟷) + 𝟼<br>
= (𝟸 𝟸) + (𝟸 𝟷) + 𝟺(𝟸 𝟷) + 𝟺(𝟸 𝟶) + 6 = 𝟻(𝟸 𝟷) + 𝟷𝟷<br>
= 𝟻(𝟷 𝟷) + 𝟻(𝟷 𝟶) + 𝟷𝟷 = 𝟸𝟷