# Matrix Multification

## Rule

Matrix A
<table style="border-spacing: 10px 0;">
  <tr>
    <td>a<sub>11</sub></td>
    <td>a<sub>12</sub></td>
  </tr>
  <tr>
    <td>a<sub>21</sub></td>
    <td>a<sub>22</sub></td>
  </tr>
</table>

Matrix B
<table style="border-spacing: 10px 0;">
  <tr>
    <td>b<sub>11</sub></td>
    <td>b<sub>12</sub></td>
  </tr>
  <tr>
    <td>b<sub>21</sub></td>
    <td>b<sub>22</sub></td>
  </tr>
</table>

Matrix C = A∙B
<table style="border-spacing: 10px 0;">
  <tr>
    <td>c<sub>11</sub> = a<sub>11</sub>∙b<sub>11</sub> + a<sub>12</sub>∙b<sub>21</sub></td>
    <td>c<sub>12</sub> = a<sub>11</sub>∙b<sub>12</sub> + a<sub>12</sub>∙b<sub>22</sub></td>
  </tr>
  <tr>
    <td>c<sub>21</sub> = a<sub>21</sub>∙b<sub>11</sub> + a<sub>22</sub>∙b<sub>21</sub></td>
    <td>c<sub>22</sub> = a<sub>21</sub>∙b<sub>12</sub> + a<sub>22</sub>∙b<sub>22</sub></td>
  </tr>
</table>

Matrix D = B∙A
<table style="border-spacing: 10px 0;">
  <tr>
    <td>d<sub>11</sub> = b<sub>11</sub>∙a<sub>11</sub> + b<sub>12</sub>∙a<sub>21</sub></td>
    <td>d<sub>12</sub> = b<sub>11</sub>∙a<sub>12</sub> + b<sub>12</sub>∙a<sub>22</sub></td>
  </tr>
  <tr>
    <td>d<sub>21</sub> = b<sub>21</sub>∙a<sub>11</sub> + b<sub>22</sub>∙a<sub>21</sub></td>
    <td>d<sub>22</sub> = b<sub>21</sub>∙a<sub>12</sub> + b<sub>22</sub>∙a<sub>22</sub></td>
  </tr>
</table>