# Function Equality

## Definition

Let &#x1D453; and &#x1D454; be functions from set &#x1D44B; into set &#x1D44C;. Then &#x1D453; = &#x1D454; if and only if &#x1D453;(&#x1D465;) = &#x1D454;(&#x1D465;) for all &#x1D465; in &#x1D44B;.

&#x1D453;, &#x1D454; : &#x1D44B; &#x2192; &#x1D44C;, &#x1D453; = &#x1D454; &#x2194; &#x1D453;(&#x1D465;) = &#x1D454;(&#x1D465;) &#x2200;&#x1D465; &#x2208; &#x1D44B;.

### Examples

- Let &#x1D453;, &#x1D454; : {-&#x1D7F7;, &#x1D7F6;, &#x1D7F7;} &#x2192; {&#x1D7F6;, &#x1D7F7;} and &#x1D453;(&#x1D465;) = |&#x1D465;|, &#x1D454;(&#x1D465;) = &#x1D465;<sup>&#x1D7F8;</sup>. Then &#x1D453; = &#x1D454;.